template-coq/theories/AstUtils.v
@@ -145,6 +145,28 @@ apply (List.firstn decl.(ind_npars)) in types.
                                                 (snd (fst x))) ind_ctors).
 Defined.
 
+Fixpoint strip_casts t :=
+  match t with
+  | tEvar ev args => tEvar ev (List.map strip_casts args)
+  | tLambda na T M => tLambda na (strip_casts T) (strip_casts M)
+  | tApp u v => mkApps (strip_casts u) (List.map (strip_casts) v)
+  | tProd na A B => tProd na (strip_casts A) (strip_casts B)
+  | tCast c kind t => strip_casts c
+  | tLetIn na b t b' => tLetIn na (strip_casts b) (strip_casts t) (strip_casts b')
+  | tCase ind p c brs =>
+    let brs' := List.map (on_snd (strip_casts)) brs in
+    tCase ind (strip_casts p) (strip_casts c) brs'
+  | tProj p c => tProj p (strip_casts c)
+  | tFix mfix idx =>
+    let mfix' := List.map (map_def strip_casts strip_casts) mfix in
+    tFix mfix' idx
+  | tCoFix mfix idx =>
+    let mfix' := List.map (map_def strip_casts strip_casts) mfix in
+    tCoFix mfix' idx
+  | tRel _ | tVar _ | tSort _ | tConst _ _ | tInd _ _ | tConstruct _ _ _ 
+  | tInt _ | tFloat _ => t
+  end.
+  
 Fixpoint decompose_prod_assum (Γ : context) (t : term) : context * term :=
   match t with
   | tProd n A B => decompose_prod_assum (Γ ,, vass n A) B
